OddOrder/Peterfalvi/S16_AppendixC3.lean
@@ -3,7 +3,8 @@ Copyright (c) 2026 Yawara Ishida. All rights reserved.
 Released under Apache 2.0 license as described in the file LICENSE.
 Authors: Yawara Ishida
 -/
-import OddOrder.Peterfalvi.S16_CoreBounds
+import OddOrder.BG.AppC_LemmaC3_ConjugateLine
+import OddOrder.Peterfalvi.S16_CoreLemmas
 
 /-!
 # S16_AppendixC3
